commit

AP/Game/Defs.lean
@@ -10,11 +10,20 @@ structure GameParams : Type (u + 1) where
   PMove : Player → Player → Type u
   Outcome : Type u
 
+  h_inh_player : Inhabited Player
   h_inh_move : ∀ p, Inhabited # Move p
   h_pl_fin : Fintype Player  
   h_pl_lin : LinearOrder Player
   h_out_lin : LinearOrder Outcome
   h_move_rfl : ∀ p, PMove p p = Move p
+
+namespace GameParams
+
+instance {T : GameParams} : Inhabited T.Player :=
+  T.h_inh_player
+
+instance {T : GameParams} {p} : Inhabited # T.Move p :=
+  T.h_inh_move p
 
 instance {T : GameParams} : Fintype T.Player :=
   T.h_pl_fin
@@ -25,39 +34,41 @@ instance {T : GameParams} : LinearOrder T.Player :=
 instance {T : GameParams} : LinearOrder T.Outcome :=
   T.h_out_lin
 
-def GameParams.Trans (T : GameParams) : Type u :=
+variable (T : GameParams)
+
+def Trans : Type u :=
   Σ (p : T.Player), T.Move p
 
-def GameParams.PTrans (T : GameParams) (p : T.Player) : Type u :=
+def PTrans (p : T.Player) : Type u :=
   Σ (p' : T.Player), T.PMove p p'
 
-def GameParams.GRules (T : GameParams) : Type u :=
+def GRules : Type u :=
   (p : T.Player) → T.State → T.Move p → Option (T.Player × T.State)
 
-abbrev GameParams.Hist (T : GameParams) : Type u :=
+abbrev Hist : Type u :=
   DMap T.Player # λ p => List (T.PTrans p)
 
 @[ext]
-structure GameParams.GState (T : GameParams) : Type u where
+structure GState : Type u where
   player : T.Player
   state : T.State
   hist : T.Hist
 
-def GameParams.initState (T : GameParams)
+def initState
 (p : T.Player) (s : T.State) : T.GState :=
   { player := p
   , state := s
   , hist := DMap.range # λ _ => []
   }
 
-def GameParams.GPMove (T : GameParams) : Type u :=
-  (p : T.Player) → T.GState → T.Trans → T.PTrans p
+def GPMove : Type u :=
+  (p : T.Player) → (s : T.GState) → T.Move s.player → T.PMove p s.player
 
-def GameParams.updateHist (T : GameParams) (pmove : T.GPMove)
+def updateHist (pmove : T.GPMove)
 (s : T.GState) (t : T.Move s.player) : T.Hist :=
-  s.hist.map # @λ p ts => pmove p s ⟨s.player, t⟩ :: ts
+  s.hist.map # @λ p ts => ⟨s.player, pmove p s t⟩ :: ts
 
-def GameParams.sys_tr (T : GameParams) (rules : T.GRules) (pmove : T.GPMove)
+def sys_tr (rules : T.GRules) (pmove : T.GPMove)
 (s : T.GState) (t : T.Trans) : Option T.GState :=
   if h : s.player = t.1 then do
     let (p₁, s₁) ← rules t.1 s.state t.2
@@ -68,17 +79,22 @@ def GameParams.sys_tr (T : GameParams) (rules : T.GRules) (pmove : T.GPMove)
       }
   else none
 
+abbrev StratFn (p : T.Player) : Type u :=
+  T.PState p → List (T.PTrans p) → T.Move p
+
+end GameParams
+
 @[ext]
 structure Game (T : GameParams) : Type u where
-  sys : System T.GState T.Trans
-  
   rules : T.GRules
   pstate : (p : T.Player) → T.State → T.PState p
   pmove : T.GPMove
-  outcome : T.GState ⊕ (ℕ → T.GState) → T.Player → T.Outcome
+  outcome : T.Player → T.State → T.Player → T.Outcome
+  
+  sys : System T.GState T.Trans
   
   h_sys_init_nemp : sys.initial ≠ ∅
-  h_sys_init_valid : ∀ s ∈ sys.initial, ∃ p s', s = T.initState p s'
+  h_sys_init_valid : ∀ s [sys.Initial s], ∃ p s', s = T.initState p s'
   h_sys_tr : sys.tr = T.sys_tr rules pmove
 
 namespace Game
@@ -90,7 +106,24 @@ def updateHist (s : T.GState) (t : T.Trans) : T.Hist :=
   then T.updateHist game.pmove s # h ▸ t.2
   else s.hist
 
-structure Strat (s₀ : T.GState) (p : T.Player) : Type u where
-  f : T.PState p → List (T.PTrans p) → T.Move p
-  h : ∀ (s : T.GState), s.player = p → game.sys.has_tr s → game.sys.valid_tr s
-    ⟨p, f (game.pstate p s.state) (s.hist.get! p)⟩
+def runStratFn {s : T.GState} (f : T.StratFn s.player) : T.Trans :=
+  let p := s.player; Sigma.mk p #
+  f (game.pstate p s.state) (s.hist.get! p)
+
+def stratCnd {p : T.Player} (f : T.StratFn p) : Prop :=
+  ∀ (s : T.GState), s.player = p → game.sys.has_tr s → game.sys.valid_tr s
+  ⟨p, f (game.pstate p s.state) (s.hist.get! p)⟩
+
+structure Strat (p : T.Player) : Type u where
+  f : T.StratFn p
+  h : game.stratCnd f
+
+def instFn (strats : ∀ p, game.Strat p) (s : T.GState) : T.Trans :=
+  game.runStratFn (strats s.player).f
+
+structure Inst : Type u where
+  strats : ∀ p, game.Strat p
+  s₀ : T.GState
+  s : T.GState
+  h_init : game.sys.Initial s₀
+  h_sim : ∃ n, game.sys.simulate (game.instFn strats) s₀ n = (s, 0)
