AP/Games/RPS/Main.lean
@@ -5,8 +5,8 @@ namespace GameRPS
 abbrev Player := Fin 2
 abbrev Item := Fin 3
 
-abbrev PlayerA : Player := 0
-abbrev PlayerB : Player := 1
+abbrev playerA : Player := 0
+abbrev playerB : Player := 1
 
 structure State where
   items : Map Player Item
@@ -17,40 +17,84 @@ abbrev Params : GameParams :=
   { Player := Player
   , State := State
   , Move := λ _ => Item
-  , PSTate := λ _ => Unit
+  , PState := λ _ => Unit
   , PMove := λ a b => if a = b then Item else Unit
   , Outcome := Bool
 
+  , h_inh_player := inferInstance
   , h_inh_move := λ _ => inferInstance
+  , h_pl_fin := inferInstance
   , h_pl_lin := inferInstance
   , h_out_lin := inferInstance
   , h_move_rfl := by simp
   }
 
-def rules : Params.Rules := λ p s t => do
+def rules : Params.GRules := λ p s t => do
   guard # s.items.get? p = none
   let s' := ⟨s.items.insert p t⟩
   return Prod.mk p.next # match s.items.get? 0 with
     | none => s'
     | some t' => if t ≠ t' then s' else State.init
 
+def pmove : Params.GPMove := λ p _ t => by
+  dsimp [GameParams.PTrans]
+  split_ifs; exact t; exact ()
+
 def RPS : Game Params :=
-  { sys :=
-    { initial := {Params.initState PlayerA State.init}
-    , tr := Params.sys_tr rules
+  { rules := rules
+  , pstate := λ _ _ => ()
+  , pmove := pmove
+  
+  , outcome := λ _ s p =>
+      ∃ x y, let items := s.items
+      items.get? p = some x ∧
+      items.get? p.next = some y ∧
+      y < x
+  
+  , sys :=
+    { initial := {Params.initState playerA State.init}
+    , tr := Params.sys_tr rules pmove
     }
   
-  , rules := rules
-  , pstate := λ _ _ => ()
-  , pmove := λ p _ ⟨p', t⟩ _ => by
-      dsimp [Params]; split_ifs; exact t; exact ()
-  
-  , outcome := λ r => match r with
-      | .inr _ => λ _ => false
-      | .inl s => λ p =>
-        let items := s.state.items
-        items.get! p.next < items.get! p
-  
-  , h_sys_initial := by simp
+  , h_sys_init_nemp := by simp
+  , h_sys_init_valid := by
+      simp [System.initial_iff]
   , h_sys_tr := rfl
+  }
+
+-----
+
+theorem stratCnd {p} {f : Params.StratFn p} : RPS.stratCnd f := by
+  rintro s h₁ ⟨⟨p, t⟩, h₂⟩
+  rw [Game.valid_tr_iff] at h₂ ⊢
+  use h₁; dsimp
+  rcases h₂ with ⟨rfl, r, h₂⟩
+  dsimp at h₂
+  simp [RPS, rules] at h₂ ⊢
+  replace h₂ := h₂.1
+  rwa [←h₁]
+
+-----
+
+def aStrat : RPS.Strat playerA :=
+  { f := λ _ _ => 1
+  , h := stratCnd
+  }
+
+def bStrat : RPS.Strat playerB :=
+  { f := λ _ _ => 0
+  , h := stratCnd
+  }
+
+def state₀ := Params.initState playerA State.init
+
+def inst : RPS.Inst :=
+  { strats := λ p => match p with
+      | 0 => aStrat
+      | 1 => bStrat
+  , s₀ := state₀
+  , s := state₀
+    
+  , h_init := ⟨rfl⟩
+  , h_sim := ⟨0, rfl⟩
   }
