AP/Game/Basic.lean
@@ -35,24 +35,44 @@ game.rules t.1 a.state t.2 = some r ∧ b =
 } := tr_eq_some_iff
 
 @[simp]
-theorem mem_hist_initState {p' p s} : p' ∈ (T.initState p s).hist := by
-  unfold GameParams.initState
-  simp
-  sorry
+theorem player_mem_hist_initState {p' p s} : p' ∈ (T.initState p s).hist := by
+  simp [GameParams.initState]
 
-#check 0 #exit
+theorem player_mem_hist_of_initial {p s} [h : game.sys.Initial s] : p ∈ s.hist := by
+  obtain ⟨p', s', rfl⟩ := game.h_sys_init_valid s
+  simp
+
+@[simp]
+theorem player_mem_updateHist_iff {p s t} :
+p ∈ game.updateHist s t ↔ p ∈ s.hist := by
+  unfold updateHist GameParams.updateHist
+  split_ifs with h₁
+  · simp
+  rfl
 
 theorem player_mem_hist_of_valid {a} [hv : game.sys.Valid a] {p} : p ∈ a.hist := by
+  classical
   cases hv
   nm s hs h
-  rcases hs with ⟨hs⟩
-  revert hs
-  induction h <;> clear s <;> intro hs
-  · nm s
-    obtain ⟨p', s', rfl⟩ := @game.h_sys_init_valid _ hs
-    simp
-
-#check 0 #exit
+  rw [System.reachable_iff_exi_trs] at h
+  obtain ⟨ts, h₁⟩ := h
+  induction ts using List.reverseRecOn generalizing a
+  · simp at h₁
+    subst h₁
+    exact game.player_mem_hist_of_initial
+  nm ts t ih
+  simp [System.trs_append] at h₁
+  iterate split at h₁ <;> simp at h₁
+  nm h₂ x s' h₃; clear x
+  rcases h₁ with ⟨rfl, h₁⟩; clear h₁
+  generalize hb : game.sys.trs s ts = b at h₂ h₃
+  specialize @ih b.1 _
+  · simp [Prod.eq_iff_fst_eq_snd_eq, hb, h₂]
+  generalize b.1 = c at h₃ ih
+  clear! b
+  rw [tr_eq_some_iff] at h₃
+  obtain ⟨h₁, r, h₂, h₃, rfl⟩ := h₃
+  simpa
 
 theorem hist_suffix_of_reachable {a} [hv : game.sys.Valid a] {b p}
 (h : game.sys.Reachable a b) : a.hist.get! p <:+ b.hist.get! p := by
@@ -67,19 +87,33 @@ theorem hist_suffix_of_reachable {a} [hv : game.sys.Valid a] {b p}
   rw [tr_eq_some_iff] at h₂
   rcases h₂ with ⟨h₂, ⟨p', c⟩, h₃, rfl⟩
   simp [Game.updateHist, GameParams.updateHist, h₂]
+  have hb := System.valid_of_reachable h₁
   rw [DMap.get!_map_eq_of_pos]
   rotate_left
-  · 
-  
-  -- exact List.suffix_cons_of_suffix ih
+  · exact game.player_mem_hist_of_valid
+  exact List.suffix_cons_of_suffix ih
 
-#check 0 #exit
-
-theorem acyclic_gstate {a} : game.sys.Acyclic a := by
+theorem acyclic_gstate {a} [ha : game.sys.Valid a] : game.sys.Acyclic a := by
   rw [System.acyclic_iff]
   intro b c t h₁ h₂ h₃
-  replace h₁ := hist_suffix_of_reachable h₁
-  replace h₃ := hist_suffix_of_reachable h₃
+  generalize (default : T.Player) = p
+  have hb := System.valid_of_reachable h₁
+  have hc : game.sys.Valid c :=
+    by
+      apply System.valid_of_reachable (a := a)
+      exact System.reachable_right h₁ h₂
+  replace h₁ := hist_suffix_of_reachable (p := p) h₁
+  replace h₃ := hist_suffix_of_reachable (p := p) h₃
   rw [tr_to_iff] at h₂
-  obtain ⟨h₂, ⟨p, t'⟩, h₄, rfl⟩:= h₂
+  obtain ⟨h₂, ⟨p', t'⟩, h₄, rfl⟩:= h₂
   simp at h₃
+  clear! p'
+  simp [updateHist, h₂, GameParams.updateHist] at h₃
+  rw [DMap.get!_map_eq_of_pos game.player_mem_hist_of_valid] at h₃
+  simp at h₃
+
+theorem valid_tr_iff {a} {t : T.Trans} :
+game.sys.valid_tr a t ↔ a.player = t.fst ∧
+∃ r, game.rules t.1 a.state t.2 = some r := by
+  simp only [System.valid_tr, System.tr_to, tr_eq_some_iff, Prod.exists,
+    exists_and_left, and_congr_right_iff]; tauto
