AP/Game/Inst.lean
@@ -1,0 +1,57 @@
+import AP.Game.Basic
+
+namespace Game.Inst
+
+variable {T : GameParams} {game : Game T} (inst : game.Inst)
+
+def f : T.GState → T.Trans :=
+  game.instFn inst.strats
+
+@[simp]
+theorem fst_f {s} : (inst.f s).fst = s.player := rfl
+
+theorem simFn_f : game.sys.SimFn inst.f := by
+  rw [System.sim_fn_iff]
+  intro s h₁
+  unfold f
+  rcases inst with ⟨f, s₀, s', h₂, h₃⟩
+  dsimp
+  clear! s₀
+  unfold Game.instFn Game.runStratFn
+  simp
+  have h₂ := (f s.player).2
+  unfold Game.stratCnd at h₂
+  exact h₂ _ rfl h₁
+
+instance : game.sys.SimFn inst.f := inst.simFn_f
+
+def step : Option game.Inst := do
+  match h : game.sys.tr inst.s (inst.f inst.s) with
+  | none => none
+  | some s' => some #
+    { inst with
+      s := s'
+    , h_sim := by
+        obtain ⟨n, h₁⟩ := inst.h_sim
+        use n + 1
+        unfold Inst.f at h
+        rw [System.simulate_add, h₁]
+        simp [h]
+    }
+
+def run (n : ℕ) : game.Inst × ℕ :=
+  match h : game.sys.simulate inst.f inst.s n with
+  | (s', m) => ((·, m)) #
+    { inst with
+      s := s'
+    , h_sim := by
+        obtain ⟨k, h₁⟩ := inst.h_sim
+        have ⟨n, hn⟩ := Nat.exists_eq_add_of_le #
+          System.snd_le_of_simulate_eq h
+        subst hn
+        use k + n
+        rw [System.simulate_add, h₁]
+        simp
+        rw [System.simulate_add_eq_left_iff] at h
+        exact h.1
+    }
