AP/Game/Main.lean
@@ -1,1 +1,1 @@
-import AP.Game.Basic
+import AP.Game.Inst
